update

test/LookupTest.lean
@@ -28,9 +28,11 @@ def lookupCircuit : Ast.Circuit := {
   ident_i := "i",
   width   := 2,
   goal    := Ast.Ty.refin Ast.Ty.unit
-    (Ast.Predicate.ind
-      (Ast.Expr.binRel (Ast.Expr.arrIdx (Ast.Expr.arrIdx (Ast.Expr.var "trace") (Ast.Expr.var "i")) (Ast.Expr.constZ 0))
-                       Ast.RelOp.eq (Ast.Expr.constF 2))),
+    (Ast.Predicate.and
+      (Ast.Predicate.ind (Ast.Expr.binRel (Ast.Expr.arrIdx (Ast.Expr.arrIdx (Ast.Expr.var "trace'") (Ast.Expr.var "i'")) (Ast.Expr.constZ 1))
+                       Ast.RelOp.eq (Ast.Expr.constF 2)))
+      (Ast.Predicate.ind (Ast.exprEq (Ast.Expr.arrIdx (Ast.Expr.arrIdx (Ast.Expr.var "trace") (Ast.Expr.var "i")) (Ast.Expr.constZ 0))
+                                     (Ast.Expr.arrIdx (Ast.Expr.arrIdx (Ast.Expr.var "trace") (Ast.Expr.var "i")) (Ast.Expr.constZ 1))))),
   body    := (Ast.Expr.lookup "assert" [((Ast.Expr.arrIdx (Ast.Expr.arrIdx (Ast.Expr.var "trace") (Ast.Expr.var "i")) (Ast.Expr.constZ 0)), (Ast.Expr.arrIdx (Ast.Expr.arrIdx (Ast.Expr.var "trace") (Ast.Expr.var "i")) (Ast.Expr.constZ 1)))])
 }
 
@@ -39,119 +41,16 @@ def Δ : Env.CircuitEnv := [("assert", assertCircuit), ("lookup", lookupCircuit)
 
 theorem lookupCircuit_correct : Ty.circuitCorrect Δ lookupCircuit 1 := by
   unfold Ty.circuitCorrect
-  intro x i height hs hi ht hσ
-  let envs := Ty.makeEnvs assertCircuit (Ast.Value.vArr x) (Ast.Value.vZ i) height
+  intro x i hs hi hrow ht
+  let envs := Ty.makeEnvs assertCircuit (Ast.Value.vArr x) (Ast.Value.vZ i) x.length
   let σ := envs.1
   let Γ := envs.2
   unfold lookupCircuit
   simp_all
-  apply Ty.TypeJudgment.TE_SUB
-  apply Ty.SubtypeJudgment.TSub_Refine
-  apply Ty.SubtypeJudgment.TSub_Refl
-  intro v
-  intro h₁
-  intro h₂
-  unfold PropSemantics.predToProp
-  unfold PropSemantics.exprToProp
-  apply Eval.EvalProp.Rel
-  apply Eval.EvalProp.ArrIdx
-  apply Eval.EvalProp.ArrIdx
-  apply Eval.EvalProp.Var
-  unfold Env.lookupVal
-  unfold Env.updateVal
-  simp
-  rfl
-  apply Eval.EvalProp.Var
-  unfold Env.lookupVal
-  unfold Env.updateVal
-  simp
-  rfl
-  unfold PropSemantics.tyenvToProp at h₁
-  u
-
+  intro h
   apply Ty.TypeJudgment.TE_LookUp
   rfl
   rfl
-  have h₁: Ast.renameVarinPred
-        (Ast.Predicate.ind
-          ((((Ast.Expr.var "trace").arrIdx (Ast.Expr.var "i")).arrIdx (Ast.Expr.constZ 1)).binRel Ast.RelOp.eq
-            (Ast.Expr.constF 2)))
-        (Env.lookupCircuit Δ "assert").ident_t (Env.freshName ["trace", "i"] (Env.lookupCircuit Δ "assert").ident_t) = (Ast.Predicate.ind
-          ((((Ast.Expr.var "trace'").arrIdx (Ast.Expr.var "i")).arrIdx (Ast.Expr.constZ 1)).binRel Ast.RelOp.eq
-            (Ast.Expr.constF 2))) := by {
-                unfold Ast.renameVarinPred
-                simp
-                unfold Ast.renameVar
-                unfold Env.freshName
-                simp
-                unfold Ast.renameVar
-                simp
-                unfold Ast.renameVar
-                simp
-                unfold Ast.renameVar
-                simp
-                unfold Env.lookupCircuit
-                unfold Δ
-                simp
-            }
-  rw[h₁]
-  have le : List.foldl (fun acc y ↦ acc.and (Ast.Predicate.ind (Ast.exprEq y.1 y.2)))
-    (Ast.renameVarinPred
-      (Ast.renameVarinPred
-        (Ast.Predicate.ind
-          ((((Ast.Expr.var "trace").arrIdx (Ast.Expr.var "i")).arrIdx (Ast.Expr.constZ 1)).binRel Ast.RelOp.eq
-            (Ast.Expr.constF 2)))
-        (Env.lookupCircuit Δ "assert").ident_t (Env.freshName ["trace", "i"] (Env.lookupCircuit Δ "assert").ident_t))
-      (Env.lookupCircuit Δ "assert").ident_i (Env.freshName ["trace", "i"] (Env.lookupCircuit Δ "assert").ident_i))
-    [(((Ast.Expr.var "trace").arrIdx (Ast.Expr.var "i")).arrIdx (Ast.Expr.constZ 0),
-        ((Ast.Expr.var "trace").arrIdx (Ast.Expr.var "i")).arrIdx (Ast.Expr.constZ 1))]
-    = (Ast.Predicate.ind
-        ((((Ast.Expr.var "trace'").arrIdx (Ast.Expr.var "i'")).arrIdx (Ast.Expr.constZ 1)).binRel Ast.RelOp.eq
-          (Ast.Expr.constF 2))) := by {
-            unfold Ast.renameVarinPred
-            unfold Ast.renameVarinPred
-            unfold Ast.renameVar
-            unfold Ast.renameVar
-
-          }
-  unfold Ast.renameVarinPred at le
-  unfold List.foldl at le
-
-  unfold Ast.renameVar at le
-  simp
-  intro h₁
-  intro h₂
-  simp
-
-  apply Ty.TypeJudgment.TE_SUB
-  apply Ty.SubtypeJudgment.TSub_Refine
-  apply Ty.SubtypeJudgment.TSub_Refl
-  intro v
-  intro h₁
-  intro h₂
-  unfold PropSemantics.predToProp at h₂
-
-  unfold PropSemantics.predToProp
-  unfold PropSemantics.exprToProp
-  apply Eval.EvalProp.Rel
-  apply Eval.EvalProp.ArrIdx
-  apply Eval.EvalProp.ArrIdx
-  apply Eval.EvalProp.Var
-  unfold Env.lookupVal
-  unfold Env.updateVal
-  simp
-  rfl
-  apply Eval.EvalProp.Var
-  unfold Env.lookupVal
-  unfold Env.updateVal
-  simp
-  rfl
-  sorry
-  apply Eval.EvalProp.ConstZ
-  sorry
-  sorry
-  apply Eval.EvalProp.ConstF
-  sorry
-  sorry
-  sorry
-  sorry
+  repeat unfold Ast.renameVarinPred; simp
+  repeat unfold Env.freshName Ast.renameVar Env.lookupCircuit Δ; simp
+  repeat unfold Ast.renameVar; simp
